base.v
@@ -40,3 +40,15 @@ Notation "A || B @ X 'by' <- H"
 *)
 Notation "A =:= B"
   := (eq_refl A : A = B) (at level 90).
+
+(**
+  Proves that every boolean value is either true
+  or false.
+*)
+Theorem bool_dec0
+  :  forall b : bool, {b = true}+{b = false}.
+Proof
+  bool_rect
+    (fun b => {b = true}+{b = false})
+       (left (true = false) (eq_refl true))
+       (right (false = true) (eq_refl false)).
